Splinter/AllocationsLayer/CoordinationBetree.dfy
@@ -1,0 +1,201 @@
+// Copyright 2018-2021 VMware, Inc., Microsoft Inc., Carnegie Mellon University, ETH Zurich, and University of Washington
+// SPDX-License-Identifier: BSD-2-Clause
+
+include "AllocationBetree.i.dfy"
+
+module CoordinationBetreeMod {
+  import opened ValueMessage
+  import opened KeyType
+  import opened StampedMod
+  import opened MsgHistoryMod
+  import opened LSNMod
+  import opened Options
+
+  import GenericDisk
+  import AllocBetree = AllocationBetreeMod
+  
+  type Address = GenericDisk.Address
+  type AU = GenericDisk.AU
+
+  datatype TransitionLabel =
+    | LoadEphemeralFromPersistentLabel(endLsn: LSN)
+    | PutRecordsLabel(records: MsgHistory)
+    | QueryLabel(endLsn: LSN, key: Key, value: Value)
+    | InternalLabel()
+    | InternalAllocationsLabel(allocs: set<AU>, deallocs: set<AU>)
+    | CommitStartLabel(newBoundaryLsn: LSN, unobserved: set<AU>)
+    | CommitCompleteLabel()
+    | CrashLabel()
+  {
+    predicate WF() {
+      && (PutRecordsLabel? ==> records.WF())
+    }
+  }
+
+  type StampedBetree = AllocBetree.StampedBetree
+
+  datatype Ephemeral =
+      | Unknown  // This means None
+      | Known(v: AllocBetree.Variables)
+
+  datatype InFlight = InFlight(
+    image: StampedBetree, // image of the stamped betree
+    freeset: set<AU>   // AUs that are allocated to betree but not yet observed, would be seen as free upon a crash
+  )
+
+  datatype Variables = Variables(
+    persistent: StampedBetree,
+    ephemeral: Ephemeral,
+    inFlight: Option<InFlight>
+  )
+  {
+    predicate WF() {
+      true
+    }
+  }
+
+  predicate LoadEphemeralFromPersistent(v: Variables, v': Variables, lbl: TransitionLabel)
+  {
+    && v.WF()
+    && lbl.LoadEphemeralFromPersistentLabel?
+    && v.ephemeral.Unknown?
+    && v'.ephemeral.Known?
+
+    && lbl.endLsn == v.persistent.seqEnd
+    && AllocBetree.Init(v'.ephemeral.v, v.persistent)
+    && v'.persistent == v.persistent // UNCHANGED
+    && v'.inFlight == v.inFlight // UNCHANGED
+  }
+
+  predicate PutRecords(v: Variables, v': Variables, lbl: TransitionLabel)
+  {
+    && v.WF()
+    && lbl.WF()
+    && lbl.PutRecordsLabel?
+    && v.ephemeral.Known?
+    && v'.ephemeral.Known?
+  
+    && AllocBetree.Next(v.ephemeral.v, v'.ephemeral.v, AllocBetree.PutLabel(lbl.records))
+    && v'.persistent == v.persistent // UNCHANGED
+    && v'.inFlight == v.inFlight // UNCHANGED
+  }
+
+  predicate Query(v: Variables, v': Variables, lbl: TransitionLabel)
+  {
+    && v.WF()
+    && lbl.WF()
+    && lbl.QueryLabel?
+    && v.ephemeral.Known?
+    && v'.ephemeral.Known?
+
+    && AllocBetree.Next(v.ephemeral.v, v'.ephemeral.v, AllocBetree.QueryLabel(lbl.endLsn, lbl.key, lbl.value))
+    && v' == v
+  }
+
+  predicate FreezeMapInternal(v: Variables, v': Variables, lbl: TransitionLabel, frozenBetree: StampedBetree, unobserved: set<AU>)
+  {
+    && v.WF()
+    && lbl.WF()
+    && lbl.InternalLabel?
+    && v.ephemeral.Known?
+    && v'.ephemeral.Known?
+
+    // Can't re-freeze until last in flight state reaches CommitComplete, since
+    // an async superblock write may be in progress, and we need to maintain
+    // guarantees about its in-flight map state.
+    && v.inFlight.None?
+    && AllocBetree.FreezeAs(v.ephemeral.v, v'.ephemeral.v, AllocBetree.FreezeAsLabel(frozenBetree, unobserved))
+    && v'.inFlight == Some(InFlight(frozenBetree, unobserved))
+    && v'.persistent == v.persistent // UNCHANGED
+  }
+  
+  predicate EphemeralInternal(v: Variables, v': Variables, lbl: TransitionLabel)
+  {
+    && v.WF()
+    && lbl.WF()
+    && lbl.InternalAllocationsLabel?
+    && v.ephemeral.Known?
+    && v'.ephemeral.Known?
+
+    && AllocBetree.Next(v.ephemeral.v, v'.ephemeral.v, AllocBetree.InternalAllocationsLabel(lbl.allocs, lbl.deallocs))
+    && v'.persistent == v.persistent // UNCHANGED
+    && v'.inFlight == v.inFlight // UNCHANGED
+  }
+
+  predicate CommitStart(v: Variables, v': Variables, lbl: TransitionLabel)
+  {
+    && v.WF()
+    && lbl.WF()
+    && lbl.CommitStartLabel?
+    && v.ephemeral.Known?
+    && v.inFlight.Some?
+
+    // Frozen map can't go backwards vs persistent map, lest we end up with
+    // a gap to the ephemeral journal start.
+    && v.persistent.seqEnd <= lbl.newBoundaryLsn
+    // Frozen journal & frozen map agree on boundary.
+    && lbl.newBoundaryLsn == v.inFlight.value.image.seqEnd
+    && lbl.unobserved == v.inFlight.value.freeset
+
+    && v' == v
+  }
+
+  predicate CommitComplete(v: Variables, v': Variables, lbl: TransitionLabel)
+  {
+    && v.WF()
+    && lbl.WF()
+    && lbl.CommitCompleteLabel?
+    && v.inFlight.Some?
+
+    && v' == v.(
+      persistent := v.inFlight.value.image,
+      // ephemeral unchanged
+      inFlight := None)
+  }
+
+  predicate Crash(v: Variables, v': Variables, lbl: TransitionLabel)
+  {
+    && v.WF()
+    && lbl.WF()
+    && lbl.CrashLabel?
+    && v' == v.(
+      ephemeral := Unknown,
+      inFlight := None)
+  }
+
+  datatype Step =
+    | LoadEphemeralFromPersistentStep()
+    | PutRecordsStep()
+    | QueryStep()
+    | FreezeMapInternalStep(frozenBetree: StampedBetree, unobserved: set<AU>)
+    | EphemeralInternalStep()
+    | CommitStartStep()
+    | CommitCompleteStep()
+    | CrashStep()
+
+
+  // Models mkfs
+  predicate Init(v: Variables)
+  {
+    v == Variables(AllocBetree.EmptyImage(), Unknown, None)
+  }
+
+  predicate NextStep(v: Variables, v': Variables, lbl: TransitionLabel, step: Step)
+  {
+    match step {
+      case LoadEphemeralFromPersistentStep() => LoadEphemeralFromPersistent(v, v', lbl)
+      case PutRecordsStep() => PutRecords(v, v', lbl)
+      case QueryStep() => Query(v, v', lbl)
+      case FreezeMapInternalStep(frozenBetree, unobserved) => FreezeMapInternal(v, v', lbl, frozenBetree, unobserved)
+      case EphemeralInternalStep() => EphemeralInternal(v, v', lbl)
+      case CommitStartStep() => CommitStart(v, v', lbl)
+      case CommitCompleteStep() => CommitComplete(v, v', lbl)
+      case CrashStep() => Crash(v, v', lbl)
+    }
+  }
+
+  predicate Next(v: Variables, v': Variables, lbl: TransitionLabel)
+  {
+    exists step :: NextStep(v, v', lbl, step)
+  }
+}
