Splinter/AllocationsLayer/MiniAllocator.i.dfy
@@ -109,13 +109,13 @@ module MiniAllocatorMod {
       && (curr.Some? ==> curr.value in allocs)
     }
 
-    function GetAllReserved() : (out: set<Address>) {
-      UnionSetOfSets(set au: AU | au in allocs :: allocs[au].reserved)
-    }
+    // function GetAllReserved() : (out: set<Address>) {
+    //   UnionSetOfSets(set au: AU | au in allocs :: allocs[au].reserved)
+    // }
 
-    function GetAllReservedAU() : (out: set<AU>) {
-      set au | au in allocs && allocs[au].reserved != {} :: au
-    }
+    // function GetAllReservedAU() : (out: set<AU>) {
+    //   set au | au in allocs && allocs[au].reserved != {} :: au
+    // }
 
     function AddAUs(aus: set<AU>) : (out: MiniAllocator)
       requires WF()
